@prefix : <http://www.semanticweb.org/tal/ontologies/llm#> .
@prefix org: <https://www.w3.org/ns/org#> .
@prefix owl: <http://www.w3.org/2002/07/owl#> .
@prefix rdf: <http://www.w3.org/1999/02/22-rdf-syntax-ns#> .
@prefix xml: <http://www.w3.org/XML/1998/namespace> .
@prefix xsd: <http://www.w3.org/2001/XMLSchema#> .
@prefix rdfs: <http://www.w3.org/2000/01/rdf-schema#> .
@prefix green-ai: <https://w3id.org/Green-AI-Ontology/ontology/> .
@base <http://www.semanticweb.org/tal/ontologies/llm#> .

<http://www.semanticweb.org/tal/ontologies/llm> rdf:type owl:Ontology ;
                                                 owl:imports <https://w3id.org/Green-AI-Ontology/ontology#> .

#################################################################
#    Annotation properties
#################################################################

###  https://w3id.org/Green-AI-Ontology/ontology/hasOperatingSystem
green-ai:hasOperatingSystem rdf:type owl:AnnotationProperty .


###  https://w3id.org/Green-AI-Ontology/ontology/hasProgrammingLanguage
green-ai:hasProgrammingLanguage rdf:type owl:AnnotationProperty .


#################################################################
#    Object Properties
#################################################################

###  http://www.semanticweb.org/tal/ontologies/llm#designedBy
:designedBy rdf:type owl:ObjectProperty ;
            rdfs:domain :AIsystem ;
            rdfs:range :Organization ;
            rdfs:comment "Links an AI system to the Organization that designed it." ;
            rdfs:label "designedBy" .


###  http://www.semanticweb.org/tal/ontologies/llm#hasEnergyMetrics
:hasEnergyMetrics rdf:type owl:ObjectProperty ;
                  rdfs:domain :LLM ;
                  rdfs:range :LLMEnergyMetrics ;
                  rdfs:comment "Associates an LLM with its Energy Metrics." ;
                  rdfs:label "hasEnergyMetrics" .


###  http://www.semanticweb.org/tal/ontologies/llm#hasEvaluation
:hasEvaluation rdf:type owl:ObjectProperty ;
               rdfs:domain :AIsystem ;
               rdfs:range :Evaluation ;
               rdfs:comment "Associates an AI system with its Evaluation criteria or results." ;
               rdfs:label "hasEvaluation" .


###  http://www.semanticweb.org/tal/ontologies/llm#hasFinetuningTask
:hasFinetuningTask rdf:type owl:ObjectProperty ;
                   rdfs:subPropertyOf :performsTask ;
                   rdfs:domain :LLM ;
                   rdfs:range :FinetuningTask ;
                   rdfs:comment "Links an LLM to its Finetuning Task." ;
                   rdfs:label "hasFinetuningTask" .


###  http://www.semanticweb.org/tal/ontologies/llm#hasHardwareSettings
:hasHardwareSettings rdf:type owl:ObjectProperty ;
                     rdfs:domain :LLM ;
                     rdfs:range :LLMHardwareSettings ;
                     rdfs:comment "Links an LLM to its Hardware Settings." ;
                     rdfs:label "hasHardwareSettings" .


###  http://www.semanticweb.org/tal/ontologies/llm#hasInferenceTask
:hasInferenceTask rdf:type owl:ObjectProperty ;
                  rdfs:subPropertyOf :performsTask ;
                  rdfs:domain :LLM ;
                  rdfs:range :InferenceTask ;
                  rdfs:comment "Links an LLM to its Inference Task." ;
                  rdfs:label "hasInferenceTask" .


###  http://www.semanticweb.org/tal/ontologies/llm#hasPretrainingTask
:hasPretrainingTask rdf:type owl:ObjectProperty ;
                    rdfs:subPropertyOf :performsTask ;
                    rdfs:domain :LLM ;
                    rdfs:range :PretrainingTask ;
                    rdfs:comment "Links an LLM to its Pretraining Task." ;
                    rdfs:label "hasPretrainingTask" .


###  http://www.semanticweb.org/tal/ontologies/llm#hasScore
:hasScore rdf:type owl:ObjectProperty ;
          rdfs:domain :Evaluation ;
          rdfs:range :Score ;
          rdfs:comment "Links an Evaluation to its Score." ;
          rdfs:label "hasScore" .


###  http://www.semanticweb.org/tal/ontologies/llm#hasSoftwareSettings
:hasSoftwareSettings rdf:type owl:ObjectProperty ;
                     rdfs:domain :LLM ;
                     rdfs:range :LLMSoftwareSettings ;
                     rdfs:comment "Links an LLM to its Software Settings." ;
                     rdfs:label "hasSoftwareSettings" .


###  http://www.semanticweb.org/tal/ontologies/llm#isCalculatedBy
:isCalculatedBy rdf:type owl:ObjectProperty ;
                rdfs:domain :Score ;
                rdfs:range :Metric ;
                rdfs:comment "Specifies the Metric used to calculate a Score." ;
                rdfs:label "isCalculatedBy" .


###  http://www.semanticweb.org/tal/ontologies/llm#performsTask
:performsTask rdf:type owl:ObjectProperty ;
              rdfs:domain :LanguageModel ;
              rdfs:range :Task ;
              rdfs:comment "Associates a Language Model with a Task it performs." ;
              rdfs:label "performsTask" .


###  http://www.semanticweb.org/tal/ontologies/llm#uses
:uses rdf:type owl:ObjectProperty ,
               owl:TransitiveProperty ;
      rdfs:domain [ rdf:type owl:Class ;
                    owl:unionOf ( :Evaluation
                                  :LLM
                                  :LLMArchitecture
                                  :TransformerComponent
                                )
                  ] ;
      rdfs:range [ rdf:type owl:Class ;
                   owl:unionOf ( <http://ontology.ethereal.cz/irao/Dataset>
                                 :LLMArchitecture
                                 :Module
                                 :TransformerComponent
                               )
                 ] ;
      rdfs:comment "A transitive property linking Evaluations, LLMs, Architectures, and Transformer Components to the Datasets, Architectures, Modules, or Transformer Components they utilize." ;
      rdfs:label "uses" .


#################################################################
#    Data properties
#################################################################

###  http://www.semanticweb.org/tal/ontologies/llm#scoreIsOf
:scoreIsOf rdf:type owl:DatatypeProperty ;
           rdfs:domain :Score ;
           rdfs:range xsd:float ;
           rdfs:comment "Associates a Score with its numeric value (float)." ;
           rdfs:label "scoreIsOf" .


#################################################################
#    Classes
#################################################################

###  http://www.semanticweb.org/tal/ontologies/llm#AIsystem
:AIsystem rdf:type owl:Class ;
          owl:equivalentClass green-ai:AIModel ;
          rdfs:comment "A general class representing an Artificial Intelligence system, equivalent to AIModel in Green-AI ontology." ;
          rdfs:label "AIsystem" .


###  http://www.semanticweb.org/tal/ontologies/llm#BERT
:BERT rdf:type owl:Class ;
      rdfs:subClassOf :LLM ;
      rdfs:comment "BERT is a subclass of Large Language Models (LLM)." ;
      rdfs:label "BERT" .


###  http://www.semanticweb.org/tal/ontologies/llm#Evaluation
:Evaluation rdf:type owl:Class ;
            rdfs:comment "Represents the evaluation metrics or criteria used to assess an AI system." ;
            rdfs:label "Evaluation" .


###  http://www.semanticweb.org/tal/ontologies/llm#FinetuningTask
:FinetuningTask rdf:type owl:Class ;
                rdfs:subClassOf :Task ;
                rdfs:comment "A specific type of Task focused on the finetuning phase of an LLM." ;
                rdfs:label "FinetuningTask" .


###  http://www.semanticweb.org/tal/ontologies/llm#GPT
:GPT rdf:type owl:Class ;
     rdfs:subClassOf :LLM ;
     rdfs:comment "Generative Pre-trained Transformer, a subclass of Large Language Models (LLM)." ;
     rdfs:label "GPT" .


###  http://www.semanticweb.org/tal/ontologies/llm#InferenceTask
:InferenceTask rdf:type owl:Class ;
               rdfs:subClassOf :Task ;
               rdfs:comment "A specific type of Task focused on the inference phase of an LLM." ;
               rdfs:label "InferenceTask" .


###  http://www.semanticweb.org/tal/ontologies/llm#LLM
:LLM rdf:type owl:Class ;
     owl:equivalentClass [ owl:intersectionOf ( :LanguageModel
                                                [ rdf:type owl:Restriction ;
                                                  owl:onProperty green-ai:hasParameters ;
                                                  owl:someValuesFrom [ rdf:type rdfs:Datatype ;
                                                                       owl:onDatatype xsd:integer ;
                                                                       owl:withRestrictions ( [ xsd:minInclusive 1000000000
                                                                                              ]
                                                                                            )
                                                                     ]
                                                ]
                                              ) ;
                           rdf:type owl:Class
                         ] ;
     rdfs:subClassOf :LanguageModel ;
     owl:disjointWith :SLM ;
     rdfs:comment "Large Language Model, a subclass of LanguageModel with a parameter count above 1 billion." ;
     rdfs:label "LLM" .


###  http://www.semanticweb.org/tal/ontologies/llm#LLMArchitecture
:LLMArchitecture rdf:type owl:Class ;
                 rdfs:comment "Represents the architectural design of a Large Language Model." ;
                 rdfs:label "LLMArchitecture" .


###  http://www.semanticweb.org/tal/ontologies/llm#LLMEnergyMetrics
:LLMEnergyMetrics rdf:type owl:Class ;
                  rdfs:subClassOf green-ai:EnergyMeasure ;
                  rdfs:comment "Energy metrics associated with a Large Language Model, subclass of EnergyMeasure from Green-AI ontology." ;
                  rdfs:label "LLMEnergyMetrics" .


###  http://www.semanticweb.org/tal/ontologies/llm#LLMHardwareSettings
:LLMHardwareSettings rdf:type owl:Class ;
                     rdfs:subClassOf green-ai:HardwareSettings ;
                     rdfs:comment "Hardware configuration settings for a Large Language Model, subclass of HardwareSettings from Green-AI ontology." ;
                     rdfs:label "LLMHardwareSettings" .


###  http://www.semanticweb.org/tal/ontologies/llm#LLMSoftwareSettings
:LLMSoftwareSettings rdf:type owl:Class ;
                     rdfs:subClassOf green-ai:SoftwareSettings ;
                     rdfs:comment "Software configuration settings for a Large Language Model, subclass of SoftwareSettings from Green-AI ontology." ;
                     rdfs:label "LLMSoftwareSettings" .


###  http://www.semanticweb.org/tal/ontologies/llm#LanguageModel
:LanguageModel rdf:type owl:Class ;
               rdfs:subClassOf :AIsystem ;
               rdfs:comment "A general class for models that process and generate human language, subclass of AI system." ;
               rdfs:label "LanguageModel" .


###  http://www.semanticweb.org/tal/ontologies/llm#MLLM
:MLLM rdf:type owl:Class ;
      rdfs:subClassOf :LLM ;
      rdfs:comment "Multi Modal Large Language Model, a subclass of LLM." ;
      rdfs:label "MLLM" .


###  http://www.semanticweb.org/tal/ontologies/llm#Metric
:Metric rdf:type owl:Class ;
        rdfs:comment "Represents a quantitative measure used to evaluate the performance or characteristics of an AI system." ;
        rdfs:label "Metric" .


###  http://www.semanticweb.org/tal/ontologies/llm#Module
:Module rdf:type owl:Class ;
        rdfs:comment "A component or unit of an LLM's architecture." ;
        rdfs:label "Module" .


###  http://www.semanticweb.org/tal/ontologies/llm#Organization
:Organization rdf:type owl:Class ;
              owl:equivalentClass org:Organization ;
              rdfs:comment "Represents an organization entity, equivalent to the Organization class in the W3 org ontology." ;
              rdfs:label "Organization" .


###  http://www.semanticweb.org/tal/ontologies/llm#PretrainingTask
:PretrainingTask rdf:type owl:Class ;
                 rdfs:subClassOf :Task ;
                 rdfs:comment "A specific type of Task focused on the pretraining phase of an LLM." ;
                 rdfs:label "PretrainingTask" .


###  http://www.semanticweb.org/tal/ontologies/llm#SLM
:SLM rdf:type owl:Class ;
     owl:equivalentClass [ owl:intersectionOf ( :LanguageModel
                                                [ rdf:type owl:Restriction ;
                                                  owl:onProperty green-ai:hasParameters ;
                                                  owl:someValuesFrom [ rdf:type rdfs:Datatype ;
                                                                       owl:onDatatype xsd:integer ;
                                                                       owl:withRestrictions ( [ xsd:maxExclusive 1000000000
                                                                                              ]
                                                                                            )
                                                                     ]
                                                ]
                                              ) ;
                           rdf:type owl:Class
                         ] ;
     rdfs:subClassOf :LanguageModel ;
     rdfs:comment "Small Language Model, a subclass of LanguageModel with a parameter count below 1 billion." ;
     rdfs:label "SLM" .


###  http://www.semanticweb.org/tal/ontologies/llm#Score
:Score rdf:type owl:Class ;
       rdfs:comment "A numerical representation of an Evaluation measure for an AI system." ;
       rdfs:label "Score" .


###  http://www.semanticweb.org/tal/ontologies/llm#Task
:Task rdf:type owl:Class ;
      rdfs:comment "Represents a task or function performed by an AI system." ;
      rdfs:label "Task" .


###  http://www.semanticweb.org/tal/ontologies/llm#TestingDataset
:TestingDataset rdf:type owl:Class ;
                rdfs:subClassOf <http://ontology.ethereal.cz/irao/Dataset> ;
                owl:disjointWith :TrainingDataset ,
                                 :ValidationDataset ;
                rdfs:comment "A dataset used for evaluating the performance of an AI system, disjoint with Training and Validation Datasets." ;
                rdfs:label "TestingDataset" .


###  http://www.semanticweb.org/tal/ontologies/llm#TrainingDataset
:TrainingDataset rdf:type owl:Class ;
                 rdfs:subClassOf <http://ontology.ethereal.cz/irao/Dataset> ;
                 owl:disjointWith :ValidationDataset ;
                 rdfs:comment "A dataset used for training an AI system, disjoint with Validation Dataset." ;
                 rdfs:label "TrainingDataset" .


###  http://www.semanticweb.org/tal/ontologies/llm#TransformerComponent
:TransformerComponent rdf:type owl:Class ;
                      rdfs:comment "This is a class of components that are specific to the Transformer architecture in an LLM." ;
                      rdfs:label "TransformerComponent" .


###  http://www.semanticweb.org/tal/ontologies/llm#ValidationDataset
:ValidationDataset rdf:type owl:Class ;
                   rdfs:subClassOf <http://ontology.ethereal.cz/irao/Dataset> ;
                   rdfs:comment "A dataset used to validate an LLM during training." ;
                   rdfs:label "ValidationDataset" .


###  https://www.w3.org/ns/org#Organization
org:Organization rdf:type owl:Class ;
                 rdfs:comment "Organization class from W3 org ontology." ;
                 rdfs:label "Organization" .


#################################################################
#    Individuals
#################################################################

###  http://www.semanticweb.org/tal/ontologies/llm#Attention
:Attention rdf:type owl:NamedIndividual ,
                    :Module ;
           rdfs:comment "An individual module representing the Attention mechanism in the Transformer architecture." ;
           rdfs:label "Attention" .


###  http://www.semanticweb.org/tal/ontologies/llm#Decoder
:Decoder rdf:type owl:NamedIndividual ,
                  :TransformerComponent ;
         rdfs:comment "An individual TransformerComponent representing the Decoder part of the Transformer architecture." ;
         rdfs:label "Decoder" .


###  http://www.semanticweb.org/tal/ontologies/llm#Encoder
:Encoder rdf:type owl:NamedIndividual ,
                  :TransformerComponent ;
         rdfs:comment "An individual TransformerComponent representing the Encoder part of the Transformer architecture." ;
         rdfs:label "Encoder" .


###  http://www.semanticweb.org/tal/ontologies/llm#FeedForward
:FeedForward rdf:type owl:NamedIndividual ,
                      :Module ;
             rdfs:comment "An individual module representing the Feed Forward network in the Transformer architecture." ;
             rdfs:label "FeedForward" .


###  http://www.semanticweb.org/tal/ontologies/llm#GPT2
:GPT2 rdf:type owl:NamedIndividual ,
               :GPT ;
      rdfs:comment "An instance of the GPT class, representing the GPT-2 model." ;
      rdfs:label "GPT2" ;
      :designedBy :OpenAI ;
      :hasEnergyMetrics :GPT2_EnergyMetrics ;
      :hasHardwareSettings :GPT2_HardwareSettings ;
      :hasSoftwareSettings :GPT2_SoftwareSettings .

###  http://www.semanticweb.org/tal/ontologies/llm#GPT2_EnergyMetrics
:GPT2_EnergyMetrics rdf:type owl:NamedIndividual ,
                             :LLMEnergyMetrics ;
                    rdfs:comment "Energy metrics for GPT2, including wattage and CO2 equivalent emissions." ;
                    rdfs:label "GPT2_EnergyMetrics" .

###  http://www.semanticweb.org/tal/ontologies/llm#GPT2_HardwareSettings
:GPT2_HardwareSettings rdf:type owl:NamedIndividual ,
                                :LLMHardwareSettings ;
                       green-ai:hasCPU :IntelCoreI7 ;
                       green-ai:hasGPU :NVIDIAGeForceRTX3070 ;
                       rdfs:comment "Hardware settings for GPT2, including CPU and GPU used." ;
                       rdfs:label "GPT2_HardwareSettings" .

###  http://www.semanticweb.org/tal/ontologies/llm#GPT2_SoftwareSettings
:GPT2_SoftwareSettings rdf:type owl:NamedIndividual ,
                                :LLMSoftwareSettings ;
                       rdfs:comment "Software settings for GPT2, including operating system and programming language." ;
                       rdfs:label "GPT2_SoftwareSettings" ;
                       green-ai:hasOperatingSystem :Ubuntu20.04 ;
                       green-ai:hasProgrammingLanguage "Python3.8" .

###  http://www.semanticweb.org/tal/ontologies/llm#GPT3
:GPT3 rdf:type owl:NamedIndividual ,
               :GPT ;
      rdfs:comment "An instance of the GPT class, representing the GPT-3 model." ;
      rdfs:label "GPT3" ;
      :designedBy :OpenAI ;
      :hasEnergyMetrics :GPT3_EnergyMetrics ;
      :hasHardwareSettings :GPT3_HardwareSettings ;
      :hasSoftwareSettings :GPT3_SoftwareSettings .

###  http://www.semanticweb.org/tal/ontologies/llm#GPT3_EnergyMetrics
:GPT3_EnergyMetrics rdf:type owl:NamedIndividual ,
                             :LLMEnergyMetrics ;
                    rdfs:comment "Energy metrics for GPT3, including wattage and CO2 equivalent emissions." ;
                    rdfs:label "GPT3_EnergyMetrics" .

###  http://www.semanticweb.org/tal/ontologies/llm#GPT3_HardwareSettings
:GPT3_HardwareSettings rdf:type owl:NamedIndividual ,
                                :LLMHardwareSettings ;
                       green-ai:hasCPU :IntelCoreI7 ;
                       green-ai:hasGPU :NVIDIAGeForceRTX3070 ;
                       rdfs:comment "Hardware settings for GPT3, including CPU and GPU used." ;
                       rdfs:label "GPT3_HardwareSettings" .

###  http://www.semanticweb.org/tal/ontologies/llm#GPT3_SoftwareSettings
:GPT3_SoftwareSettings rdf:type owl:NamedIndividual ,
                                :LLMSoftwareSettings ;
                       rdfs:comment "Software settings for GPT3, including operating system and programming language." ;
                       rdfs:label "GPT3_SoftwareSettings" ;
                       green-ai:hasOperatingSystem :Ubuntu20.04 ;
                       green-ai:hasProgrammingLanguage "Python3.8" .

###  http://www.semanticweb.org/tal/ontologies/llm#GPT4
:GPT4 rdf:type owl:NamedIndividual ,
               :GPT ;
      :designedBy :OpenAI ;
      :hasEnergyMetrics :GPT4_EnergyMetrics ;
      :hasHardwareSettings :GPT4_HardwareSettings ;
      :hasSoftwareSettings :GPT4_SoftwareSettings ;
      rdfs:comment "An instance of the GPT class, representing the GPT-4 model, along with its energy, hardware, and software settings." ;
      rdfs:label "GPT4" .


###  http://www.semanticweb.org/tal/ontologies/llm#GPT4_EnergyMetrics
:GPT4_EnergyMetrics rdf:type owl:NamedIndividual ,
                             :LLMEnergyMetrics ;
                    rdfs:comment "Energy metrics for GPT4, including wattage and CO2 equivalent emissions." ;
                    rdfs:label "GPT4_EnergyMetrics" .


###  http://www.semanticweb.org/tal/ontologies/llm#GPT4_HardwareSettings
:GPT4_HardwareSettings rdf:type owl:NamedIndividual ,
                                :LLMHardwareSettings ;
                       green-ai:hasCPU :IntelCoreI7 ;
                       green-ai:hasGPU :NVIDIAGeForceRTX3070 ;
                       rdfs:comment "Hardware settings for GPT4, including CPU and GPU used." ;
                       rdfs:label "GPT4_HardwareSettings" .


###  http://www.semanticweb.org/tal/ontologies/llm#GPT4_SoftwareSettings
:GPT4_SoftwareSettings rdf:type owl:NamedIndividual ,
                                :LLMSoftwareSettings ;
                       rdfs:comment "Software settings for GPT4, including operating system and programming language." ;
                       rdfs:label "GPT4_SoftwareSettings" ;
                       green-ai:hasOperatingSystem :Ubuntu20.04 ;
                       green-ai:hasProgrammingLanguage "Python3.8" .


###  http://www.semanticweb.org/tal/ontologies/llm#IntelCoreI7
:IntelCoreI7 rdf:type owl:NamedIndividual .


###  http://www.semanticweb.org/tal/ontologies/llm#NVIDIAGeForceRTX3070
:NVIDIAGeForceRTX3070 rdf:type owl:NamedIndividual .


###  http://www.semanticweb.org/tal/ontologies/llm#OpenAI
:OpenAI rdf:type owl:NamedIndividual ,
                 :Organization ;
        rdfs:comment "An individual Organization entity representing OpenAI." ;
        rdfs:label "OpenAI" .


###  http://www.semanticweb.org/tal/ontologies/llm#Transformer
:Transformer rdf:type owl:NamedIndividual ,
                      :LLMArchitecture ;
             rdfs:comment "An individual representing the Transformer architecture used in LLMs." ;
             rdfs:label "Transformer" .

###  http://www.semanticweb.org/tal/ontologies/llm#RoBERTa
:RoBERTa rdf:type owl:NamedIndividual,
                   :BERT ;
          rdfs:comment "An individual representing the RoBERTa model, a robustly optimized BERT model." ;
          rdfs:label "RoBERTa" ;
          :designedBy :OpenAI ;
          :hasFinetuningTask :RoBERTa_FinetuningTask ;
          green-ai:hasParameters 1200000000 ;
          green-ai:hasProgrammingLanguage "Python3.8" ;
          :hasEnergyMetrics :RoBERTa_EnergyMetrics ;
          :hasHardwareSettings :RoBERTa_HardwareSettings ;
          :hasSoftwareSettings :RoBERTa_SoftwareSettings .

###  http://www.semanticweb.org/tal/ontologies/llm#RoBERTa_FinetuningTask
:RoBERTa_FinetuningTask rdf:type owl:NamedIndividual,
                                :PretrainingTask ;
                       rdfs:comment "Finetuning task for RoBERTa, focusing on specific tasks like text classification." ;
                       rdfs:label "RoBERTa_FinetuningTask" .

###  http://www.semanticweb.org/tal/ontologies/llm#RoBERTa_EnergyMetrics
:RoBERTa_EnergyMetrics rdf:type owl:NamedIndividual,
                                :LLMEnergyMetrics ;
                       green-ai:hasWatt "120.0"^^xsd:float ;
                       green-ai:hasKgOfCO2eq "60.0"^^xsd:float .

###  http://www.semanticweb.org/tal/ontologies/llm#RoBERTa_HardwareSettings
:RoBERTa_HardwareSettings rdf:type owl:NamedIndividual,
                                :LLMHardwareSettings ;
                       green-ai:hasCPU :IntelCoreI7 ;
                       green-ai:hasGPU :NVIDIAGeForceRTX3070 ;
                       rdfs:comment "Hardware settings for RoBERTa, including CPU and GPU used." ;
                       rdfs:label "RoBERTa_HardwareSettings" .

###  http://www.semanticweb.org/tal/ontologies/llm#RoBERTa_SoftwareSettings
:RoBERTa_SoftwareSettings rdf:type owl:NamedIndividual ,
                                :LLMSoftwareSettings ;
                       rdfs:comment "Software settings for RoBERTa, including operating system and programming language." ;
                       rdfs:label "RoBERTa_SoftwareSettings" ;
                       green-ai:hasOperatingSystem :Ubuntu20.04 ;
                       green-ai:hasProgrammingLanguage "Python3.8" .

###  http://www.semanticweb.org/tal/ontologies/llm#DistilBERT
:DistilBERT rdf:type owl:NamedIndividual,
                  :BERT ;
             rdfs:comment "An individual representing the DistilBERT model, a distilled version of BERT." ;
             rdfs:label "DistilBERT" ;
             :designedBy :OpenAI ;
             :hasFinetuningTask :DistilBERT_FinetuningTask ;
             green-ai:hasParameters 1200000000 ;
             green-ai:hasProgrammingLanguage "Python3.8" ;
             :hasEnergyMetrics :DistilBERT_EnergyMetrics ;
             :hasHardwareSettings :DistilBERT_HardwareSettings ;
             :hasSoftwareSettings :DistilBERT_SoftwareSettings .

###  http://www.semanticweb.org/tal/ontologies/llm#DistilBERT_EnergyMetrics
:DistilBERT_EnergyMetrics rdf:type owl:NamedIndividual,
                                :LLMEnergyMetrics ;
                       green-ai:hasWatt "120.0"^^xsd:float ;
                       green-ai:hasKgOfCO2eq "60.0"^^xsd:float .

###  http://www.semanticweb.org/tal/ontologies/llm#DistilBERT_HardwareSettings
:DistilBERT_HardwareSettings rdf:type owl:NamedIndividual,
                                :LLMHardwareSettings ;
                       green-ai:hasCPU :IntelCoreI7 ;
                       green-ai:hasGPU :NVIDIAGeForceRTX3070 ;
                       rdfs:comment "Hardware settings for DistilBERT, including CPU and GPU used." ;
                       rdfs:label "DistilBERT_HardwareSettings" .

###  http://www.semanticweb.org/tal/ontologies/llm#DistilBERT_SoftwareSettings
:DistilBERT_SoftwareSettings rdf:type owl:NamedIndividual,
                                :LLMSoftwareSettings ;
                       rdfs:comment "Software settings for DistilBERT, including operating system and programming language." ;
                       rdfs:label "DistilBERT_SoftwareSettings" ;
                       green-ai:hasOperatingSystem :Ubuntu20.04 ;
                       green-ai:hasProgrammingLanguage "Python3.8" .

###  http://www.semanticweb.org/tal/ontologies/llm#DistilBERT_FinetuningTask
:DistilBERT_FinetuningTask rdf:type owl:NamedIndividual,
                                :PretrainingTask ;
                       rdfs:comment "Finetuning task for DistilBERT, focusing on specific tasks like text classification." ;
                       rdfs:label "DistilBERT_FinetuningTask" .

###  http://www.semanticweb.org/tal/ontologies/llm#GPT4V
:GPT4V rdf:type owl:NamedIndividual,
           :MLLM ;
         rdfs:comment "An individual representing the GPT-4 Vision model, a multimodal large language model." ;
         rdfs:label "GPT-4V" ;
         :designedBy :OpenAI ;
         :hasInferenceTask :GPT4V_InferenceTask ;
         green-ai:hasOperatingSystem "Ubuntu20.04" ;
         :hasEnergyMetrics :GPT4V_EnergyMetrics ;
         :hasHardwareSettings :GPT4V_HardwareSettings ;
         :hasSoftwareSettings :GPT4V_SoftwareSettings .

###  http://www.semanticweb.org/tal/ontologies/llm#GPT4V_InferenceTask
:GPT4V_InferenceTask rdf:type owl:NamedIndividual,
                                :InferenceTask ;
                       rdfs:comment "Inference task for GPT4V, focusing on multimodal inputs like images." ;
                       rdfs:label "GPT4V_InferenceTask" .

###  http://www.semanticweb.org/tal/ontologies/llm#GPT4V_EnergyMetrics
:GPT4V_EnergyMetrics rdf:type owl:NamedIndividual ,
                             :LLMEnergyMetrics ;
                    rdfs:comment "Energy metrics for GPT4V, including wattage and CO2 equivalent emissions." ;
                    rdfs:label "GPT4V_EnergyMetrics" .

###  http://www.semanticweb.org/tal/ontologies/llm#GPT4V_HardwareSettings
:GPT4V_HardwareSettings rdf:type owl:NamedIndividual ,
                                :LLMHardwareSettings ;
                       green-ai:hasCPU :IntelCoreI7 ;
                       green-ai:hasGPU :NVIDIAGeForceRTX3070 ;
                       rdfs:comment "Hardware settings for GPT4V, including CPU and GPU used." ;
                       rdfs:label "GPT4V_HardwareSettings" .

###  http://www.semanticweb.org/tal/ontologies/llm#GPT4V_SoftwareSettings
:GPT4V_SoftwareSettings rdf:type owl:NamedIndividual ,
                                :LLMSoftwareSettings ;
                       rdfs:comment "Software settings for GPT4V, including operating system and programming language." ;
                       rdfs:label "GPT4V_SoftwareSettings" ;
                       green-ai:hasOperatingSystem :Ubuntu20.04 ;
                       green-ai:hasProgrammingLanguage "Python3.8" .



###  Generated by the OWL API (version 4.5.29.2024-05-13T12:11:03Z) https://github.com/owlcs/owlapi
